Suppose $p$ is prime, therefore $gcd(a, p) = 1$.  

Consider the first $p - 1$ numbers: $ 1, 2, 3,..., p - 1$. They for a complete residue system, meaning that for any integer $0 \leq a, b \leq p - 1, a \not\equiv b \ (mod \ p)$.

Next, consider the first $p - 1$ multiples of $a$ : $a, 2a, 3a,...,(p - 1)a$, and notice that they also form a complete residue system. Namely, for any $a, b$ such that $ ax_1 \equiv ax_2 \ (mod \ p)$ :
$$
ax_1 \equiv ax_2 \ (\textrm{mod} \ p) \Rightarrow p|a(x_1 - x_2)\\
\Rightarrow p|x_1 - x_2\ (gcd(a, p) = 1) \Rightarrow x_1 \equiv x_2 \ (\textrm{mod} p)
$$
This means that if $x_1 \not\equiv\ x_2 \ (\textrm{mod} p)$, then $ax_1 \not\equiv ax_2 \ (\textrm{mod} \ p)$, which proves that $a, 2a, 3a,...,(p - 1)a$ forms a complete residue system. Therefore,
$$
a \cdot 2a \cdot 3a \cdot 4a \ ...\ (p - 1)a = \\
a^{p-1} \cdot (p - 1)! \equiv (p - 1)! \ (\textrm{mod} p)
$$
Since $gcd((p - 1)!, p) = 1, (p - 1)!$ can be divided from both sides, resulting in *Fermat's Little Theorem*:
$$
a^{p-1} \equiv 1 \ (\textrm{mod} p)
$$

